Remove one admit

src/examples/Kuiper.Example.IntApprox.fst
@@ -4,31 +4,45 @@ module Kuiper.Example.IntApprox
 
 open Kuiper
 open Kuiper.Seq.Common
+module SZ = Kuiper.SizeT
 module U32 = FStar.UInt32
+module Array1 = Kuiper.Array1
+open Kuiper.Tensor.Layout.Alg { l1_forward }
 
 (* Strengthen the spec of a reduction *)
 
 noextract
 fn reduce (#et:Type0) {| scalar et, real_like et |}
-  (len : erased nat) (a : larray u32 len) (#s : erased (seq u32))
-  (#r : erased (seq real))
-  preserves a |-> s ** pure (s %~ r)
+  (len : szp)
+  (a : Array1.t u32 (l1_forward len) { Array1.is_global a })
+  (#s : erased (lseq u32 len))
+  (r : erased (lseq real len))
+  preserves cpu
+  preserves on gpu_loc (a |-> s)
+  requires  pure (s %~ r) **
+            pure (SZ.fits (len + 1024sz)) // Almost impossible to falsify
   returns   res : u32
-  ensures   pure (res %~ seq_fold_left (+.) 0.0R r)
+  ensures   pure (res %~ rsum r)
 {
-  admit(); // Intentional, to not import HReduce here.
+  assert pure (Seq.equal (seq_map id r) r);
+  Kuiper.Kernel.HReduce.reduce id id 1024sz len a r;
 }
 
 (* A stronger exact spec for reduce on u32s, proven from the approximate spec. *)
 noextract
-fn reduce_u32 (len : erased nat) (a : larray u32 len) (#s : erased (seq u32))
-  preserves a |-> s
+fn reduce_u32
+  (len : szp)
+  (a : Array1.t u32 (l1_forward len) { Array1.is_global a })
+  (#s : erased (lseq u32 len))
+  preserves cpu
+  preserves on gpu_loc (a |-> s)
+  requires  pure (SZ.fits (len + 1024sz)) // Almost impossible to falsify
   returns   res : u32
   ensures   pure (U32.v res == seq_fold_left add zero s)
 {
   to_real_seq_is_approx s;
-  let res = reduce #u32 len a #s #(seq_map to_real s);
-  let rr = seq_fold_left (+.) 0.0R (seq_map to_real s);
+  let res = reduce #u32 len a #s (seq_map to_real s);
+  let rr = rsum (seq_map to_real s);
   assert pure (res %~ rr);
   sum_is_approx s (seq_map to_real s);
   v_approximates_inj res (seq_fold_left add zero s) rr;
